Nat_Show_Utils.thy
@@ -1,0 +1,146 @@
+theory Nat_Show_Utils
+imports "Show.Show_Instances"
+begin
+
+text \<open> By Maximlian Shäffeler:
+https://isabelle.zulipchat.com/#narrow/channel/238552-Beginner-Questions/topic/String.20inequality.20with.20show/near/500270718 \<close>
+
+lemma div_mod_imp_eq: \<open>(a :: nat) div n = b div n \<Longrightarrow> a mod n = b mod n \<Longrightarrow> a = b\<close>
+  by (metis div_mult_mod_eq)
+
+lemma string_of_digit_inj:
+  assumes \<open>a \<noteq> (b :: nat)\<close> \<open>a < 10\<close> \<open>b < 10\<close>
+  shows \<open>string_of_digit a \<noteq> string_of_digit b\<close>
+proof -
+  have \<open>a \<in> {0, 1, 2, 3, 4, 5, 6, 7, 8, 9}\<close>
+    using \<open>a < 10\<close>
+    by auto
+  thus ?thesis
+    using \<open>a \<noteq> b\<close> \<open>b < 10\<close>
+    by auto (auto split: if_splits simp: string_of_digit_def)
+qed
+
+lemma shows_prec_nat: \<open>shows_prec p n '''' = (if n < 10 then string_of_digit n
+    else shows_prec p (n div 10) '''' @ string_of_digit (n mod 10))\<close>
+  unfolding shows_prec_nat_def
+proof (induction p n rule: showsp_nat.induct)
+  case (1 p n)
+  then show ?case
+    unfolding shows_string_def showsp_nat.simps[of p n]
+    by (auto simp: shows_prec_append[symmetric] shows_prec_nat_def[symmetric])
+qed
+
+lemma show_nat: \<open>show n = (if n < 10 then string_of_digit n
+    else show (n div 10) @ string_of_digit (n mod 10))\<close>
+  using shows_prec_nat .
+
+lemma show_nat_induct:
+  \<open>(\<And>n. (\<And>z. \<not> n < 10 \<Longrightarrow> z \<in> range (shows_string (string_of_digit (n mod 10))) \<Longrightarrow> P (n div 10)) \<Longrightarrow> P n) \<Longrightarrow> P n\<close>
+  by (rule showsp_nat.induct) blast
+
+lemma length_string_of_digit[simp]: \<open>length (string_of_digit n) = 1\<close>
+  unfolding string_of_digit_def
+  by auto
+
+lemma len_show_ge10: \<open>(n :: nat) \<ge> 10 \<Longrightarrow> length (show n) \<ge> 2\<close>
+  unfolding show_nat[of n] show_nat[of \<open>(n div 10)\<close>]
+  by auto
+
+lemma len_show_lt10: \<open>(n :: nat) < 10 \<Longrightarrow> length (show n) = 1\<close>
+  unfolding show_nat[of n]
+  by auto
+
+lemma show_nat_inj:
+  fixes a b :: nat
+  assumes \<open>a \<noteq> b\<close>
+  shows \<open>show a \<noteq> show b\<close>
+  using assms
+proof (induction a arbitrary: b rule: show_nat_induct)
+  case (1 n)
+  hence ?case if \<open>\<not>n < 10\<close> \<open>\<not>b < 10\<close>
+    using that div_mod_imp_eq[of n 10 b] string_of_digit_inj[of \<open>n mod 10\<close> \<open>b mod 10\<close>]
+    by (cases \<open>n div 10 = b div 10\<close>) (auto simp: show_nat[of n] show_nat[of b])
+  moreover have ?case if \<open>n < 10\<close> \<open>b < 10\<close>
+    using 1 string_of_digit_inj that
+    by (auto simp: show_nat[of n] show_nat[of b])
+  moreover have ?case if \<open>((n :: nat) < 10) \<noteq> ((b :: nat) < 10)\<close>
+    using that len_show_ge10[of n] len_show_lt10[of b] len_show_ge10[of b] len_show_lt10[of n]
+    by auto
+  ultimately show ?case
+    by blast
+qed
+
+text \<open> My stuff \<close>
+
+lemma nat_induct_all [case_names 0 Suc]:
+  fixes n::nat
+  assumes "P 0" "\<And>n. (\<And>k. k \<le> n \<Longrightarrow> P k) \<Longrightarrow> P (Suc n)"
+  shows "P n"
+proof -
+  have "\<And>k. k \<le> n \<Longrightarrow> P k" by (induction n) (auto simp add: le_Suc_eq assms)
+  thus ?thesis by simp
+qed
+
+
+lemma nat_induct_10 [case_names digit0 digitN]:
+  fixes n::nat
+  assumes "(\<And>n. n < 10 \<Longrightarrow> P n)" "(\<And>n m. P n \<Longrightarrow> m < 10 \<Longrightarrow> P (10 * n + m))"
+  shows "P n"
+proof (induction n rule: nat_induct_all)
+  case (Suc n)
+  show "P (Suc n)"
+  proof (cases)
+    assume "Suc n \<ge> 10"
+    with Suc show ?thesis
+      using assms(2)[of "Suc n div 10" "Suc n mod 10"] by simp
+  qed (simp add: assms)
+qed (simp add: assms)
+
+lemma digit_chars: "set (string_of_digit n) \<subseteq> {CHR ''0'', CHR ''1'', CHR ''2'', CHR ''3'',
+  CHR ''3'', CHR ''4'', CHR ''5'', CHR ''6'', CHR ''7'', CHR ''8'', CHR ''9''}"
+  unfolding string_of_digit_def by simp
+
+lemma show_nat_chars:
+  fixes n :: nat
+  shows "set (show n) \<subseteq> {CHR ''0'', CHR ''1'', CHR ''2'', CHR ''3'',
+  CHR ''3'', CHR ''4'', CHR ''5'', CHR ''6'', CHR ''7'', CHR ''8'', CHR ''9''}"
+  apply (induction n rule: nat_induct_10)
+  using show_nat digit_chars by simp_all
+
+lemma notin_show_nat: "CHR ''_'' \<notin> set (show (n::nat))"
+  using show_nat_chars by blast
+
+lemma nat_show_len_mono:
+  fixes i j :: nat
+  assumes "i \<le> j"
+  shows "length (show i) \<le> length (show j)"
+proof -
+  have "\<And>k. k \<le> n \<Longrightarrow> length (show k) \<le> length (show (Suc k))" for n
+  proof (induction n rule: nat_induct_10)
+    case (digitN n m)
+    show ?case
+    proof (cases "k \<ge> 10")
+      case True
+      from digitN have "k div 10 \<le> n" by simp
+      with digitN have kih: "length (show (k div 10)) \<le> length (show (Suc (k div 10)))" by simp
+      have "Suc k div 10 = k div 10 \<or> Suc k div 10 = Suc (k div 10)" by auto
+      hence "show (Suc k) = show (k div 10) @ string_of_digit (Suc k mod 10) \<or>
+        show (Suc k) = show (Suc (k div 10)) @ string_of_digit (Suc k mod 10)"
+        using show_nat True by fastforce
+      with kih show ?thesis using show_nat by fastforce
+    qed (simp_all add: show_nat)
+  qed (simp add: show_nat)
+  hence "length (show n) \<le> length (show (Suc n))" for n by auto
+  hence "length (show i) \<le> length (show (i+k))" for i k :: nat
+    apply (induction k arbitrary: i)
+     apply simp
+    using le_trans by fastforce
+  thus ?thesis using assms by (metis le_iff_add)
+qed
+
+lemma nat_show_len_nonzero:
+  fixes n :: nat
+  shows "length (show n) \<ge> 1"
+  using show_nat by simp
+
+end
